src/Compilers/Named/WfFromUnit.v
@@ -1,0 +1,82 @@
+Require Import Crypto.Compilers.Syntax.
+Require Import Crypto.Compilers.Named.Context.
+Require Import Crypto.Compilers.Named.ContextProperties.
+Require Import Crypto.Compilers.Named.ContextDefinitions.
+Require Import Crypto.Compilers.Named.Syntax.
+Require Import Crypto.Compilers.Named.Wf.
+Require Import Crypto.Util.PointedProp.
+Require Import Crypto.Util.Tactics.BreakMatch.
+Require Import Crypto.Util.Tactics.SplitInContext.
+Require Import Crypto.Util.Tactics.DestructHead.
+Require Import Crypto.Util.Decidable.
+Require Import Crypto.Util.Option.
+
+Section language.
+  Context {base_type_code Name : Type}
+          {op : flat_type base_type_code -> flat_type base_type_code -> Type}
+          {base_type_code_dec : DecidableRel (@eq base_type_code)}
+          {Name_dec : DecidableRel (@eq Name)}.
+
+  Section with_var.
+    Context {var}
+            (uContext : @Context base_type_code Name (fun _ => unit))
+            (uContextOk : ContextOk uContext)
+            (vContext : @Context base_type_code Name var)
+            (vContextOk : ContextOk vContext).
+
+    Local Ltac t :=
+      repeat first [ progress simpl in *
+                   | progress intros
+                   | progress subst
+                   | progress inversion_option
+                   | congruence
+                   | tauto
+                   | solve [ eauto ]
+                   | break_innermost_match_step
+                   | break_innermost_match_hyps_step
+                   | progress destruct_head'_and
+                   | progress autorewrite with push_prop_of_option push_eq_Some_trivial in *
+                   | rewrite !(@lookupb_extend base_type_code _ Name _) by auto
+                   | rewrite (@find_Name_and_val_split base_type_code _ Name _) with (default := lookupb _ _)
+                   | match goal with
+                     | [ H : ?x = Some _ |- _ ]
+                       => assert (x = None) by (split_iff; eauto); congruence
+                     | [ |- _ /\ _ ] => split
+                     | [ H : _ |- prop_of_option _ ] => eapply H; [ | eassumption ]; clear H
+                     | [ |- context[find_Name_and_val ?tdec ?ndec ?b _ _ _ _ = None] ]
+                       => rewrite <- !(@find_Name_and_val_None_iff _ tdec _ ndec _ b)
+                     end ].
+
+    Lemma wff_from_unit
+          (vctx : vContext)
+          (uctx : uContext)
+          (Hctx : forall t n, lookupb vctx n t = None <-> lookupb uctx n t = None)
+          {t} (e : @exprf base_type_code op Name t)
+      : wff_unit uctx e = Some trivial -> prop_of_option (wff vctx e).
+    Proof using Name_dec base_type_code_dec uContextOk vContextOk.
+      revert uctx vctx Hctx; induction e; t.
+    Qed.
+
+    Lemma wf_from_unit
+          (vctx : vContext)
+          (uctx : uContext)
+          (Hctx : forall t n, lookupb vctx n t = None <-> lookupb uctx n t = None)
+          {t} (e : @expr base_type_code op Name t)
+      : wf_unit uctx e = Some trivial -> wf vctx e.
+    Proof using Name_dec base_type_code_dec uContextOk vContextOk.
+      intros H ?; revert H; apply wff_from_unit; t.
+    Qed.
+  End with_var.
+
+  Lemma Wf_from_unit
+        (Context : forall var, @Context base_type_code Name var)
+        (ContextOk : forall var, ContextOk (Context var))
+        {t} (e : @expr base_type_code op Name t)
+    : wf_unit (Context:=Context _) empty e = Some trivial -> Wf Context e.
+  Proof using Name_dec base_type_code_dec.
+    intros H ?; revert H; apply wf_from_unit; auto; intros.
+    rewrite !lookupb_empty by auto; tauto.
+  Qed.
+End language.
+
+Hint Resolve wf_from_unit Wf_from_unit wff_from_unit : wf.
